introduced a boolean function and a tactic for testing non-termination

trunk/color/NonTermin/ALoop.v
@@ -11,7 +11,7 @@ Set Implicit Arguments.
 
 Require Import NatUtil.
 Require Import ATrs.
-Require Import List.
+Require Import ListUtil.
 Require Import ListDec.
 Require Import APosition.
 Require Import LogicUtil.
@@ -22,6 +22,7 @@ Section S.
 Variable Sig : Signature.
 
 Notation term := (term Sig). Notation context := (context Sig).
+Notation substitution := (substitution Sig).
 Notation rule := (rule Sig). Notation rules := (list rule).
 
 Variable R : rules.
@@ -53,33 +54,59 @@ Defined.
 (***********************************************************************)
 (** data necessary for a sequence of rewrite steps *)
 
-Notation data := (position * rule)%type.
+Definition data := (position * rule)%type.
 
-Definition rewrite (d : data) t : option {u | red R t u}.
+Definition rewrite (t : term) (d : data) : option term :=
+  let (p,a) := d in let (l,r) := a in
+    if mem (@beq_rule Sig) (mkRule l r) R then
+      match subterm_pos t p with
+        | None => None
+        | Some u =>
+          match matches l u with
+            | None => None
+            | Some s => replace_pos t p (sub s r)
+          end
+      end
+      else None.
+
+Lemma rewrite_correct : forall t d u, rewrite t d = Some u -> red R t u.
 
 Proof.
-intros [p [l r]] t.
-case_eq (mem (@beq_rule Sig) (mkRule l r) R); [idtac|exact None].
-case_eq (subterm_pos t p); [idtac|exact None]. rename t0 into tp.
-case_eq (matches l tp); [idtac|exact None]. rename t0 into s.
-case_eq (replace_pos t p (sub s r)). apply Some. exists  t0.
-rewrite red_pos_ok. exists p. exists l. exists r. exists s.
-intuition. rewrite mem_ok in H. hyp. apply beq_rule_ok. rewrite H0.
-ded (matches_correct H1). rewrite H3. refl.
-ded (subterm_pos_replace_neq_None _ (sub s r) _ H0). rewrite H2 in H3. irrefl.
-Defined.
+intros t [p [l r]] u. unfold rewrite.
+case_eq (mem (@beq_rule Sig) (mkRule l r) R). 2: discr.
+gen H0. case_eq (subterm_pos t p). 2: discr.
+gen H1. case_eq (matches l t0). rename t1 into s. 2: discr.
+rewrite red_pos_ok. exists p. exists l. exists r. exists s. intuition.
+rewrite mem_ok in H. hyp. apply beq_rule_ok.
+ded (matches_correct H1). rewrite H3. hyp.
+Qed.
 
-Definition rewrites (ds : list data) t : option {us| FS t us}.
+Implicit Arguments rewrite_correct [t d u].
+
+Fixpoint rewrites t (ds : list data) {struct ds} : option (list term) :=
+  match ds with
+    | nil => Some nil
+    | d :: ds' =>
+      match rewrite t d with
+        | None => None
+        | Some u =>
+          match rewrites u ds' with
+            | None => None
+            | Some us => Some (u::us)
+          end
+      end
+  end.
+
+Lemma rewrites_correct : forall ds t us, rewrites t ds = Some us -> FS t us.
 
 Proof.
-induction 1.
-(* nil *)
-intro t. apply Some. exists nil. exact I.
-(* cons *)
-intro t. destruct (rewrite a t); [idtac|exact None].
-destruct s. destruct (IHds x); [idtac|exact None]. destruct s.
-apply Some. exists (x :: x0). simpl. intuition.
-Defined.
+induction ds; simpl; intros. inversion H. exact I.
+gen H. case_eq (rewrite t a). 2: discr.
+gen H0. case_eq (rewrites t0 ds). 2: discr.
+inversion H1. simpl. ded (rewrite_correct H). intuition.
+Qed.
+
+Implicit Arguments rewrites_correct [ds t us].
 
 Lemma FS_red : forall ts t, FS t ts -> forall i,
   i < length ts -> red R (nth i (t::ts) (Var 0)) (nth (S i) (t::ts) (Var 0)).
@@ -92,13 +119,14 @@ Qed.
 (***********************************************************************)
 (** assumptions for non-termination *)
 
-Variables (t : term) (r : {us|FS t us}).
+Section loop.
 
-Definition list_terms := terms_of_reduc r.
+Variables (t : term) (ds : list data)
+  (us : list term) (h1 : rewrites t ds = Some us).
 
-Definition k := length list_terms.
+Definition k := length us.
 
-Definition nth i := nth i list_terms (Var 0).
+Definition nth i := nth i us (Var 0).
 
 Definition last_term := nth (k-1).
 
@@ -107,15 +135,18 @@ Variables (h0 : k > 0).
 Lemma FS_red' : forall i, i < k - 1 -> red R (nth i) (nth (S i)).
 
 Proof.
-intros. unfold nth, list_terms.
-change (red R (List.nth (S i) (t :: terms_of_reduc r) (Var 0))
-  (List.nth (S (S i)) (t :: terms_of_reduc r) (Var 0))).
-apply FS_red. destruct r. hyp. unfold k, list_terms in *. omega.
+intros. unfold nth.
+change (red R (List.nth (S i) (t :: us) (Var 0))
+  (List.nth (S (S i)) (t :: us) (Var 0))).
+apply FS_red. eapply rewrites_correct. apply h1. unfold k in *. omega.
 Qed.
 
-Variables (ds : list data) (h1 : rewrites ds t = Some r)
-  (p : position) (u : term) (h2 : subterm_pos last_term p = Some u)
-  (s : substitution Sig) (h3 : matches t u = Some s).
+Variables (p : position) (u : term) (h2 : subterm_pos last_term p = Some u)
+  (s : substitution) (h3 : matches t u = Some s).
+
+(***********************************************************************)
+(** proof of non-termination *)
+
 Definition c : context.
 
 Proof.
@@ -135,7 +166,7 @@ Lemma red_g : forall a b, red R a b -> red R (g a) (g b).
 
 Proof.
 intros. redtac. unfold red. unfold g.
-exists l. exists r0. exists (AContext.comp c (subc s c0)). exists (comp s s0).
+exists l. exists r. exists (AContext.comp c (subc s c0)). exists (comp s s0).
 subst. repeat rewrite sub_fill. repeat rewrite fill_comp.
 repeat rewrite sub_sub. intuition.
 Qed.
@@ -153,7 +184,7 @@ Require Import Euclid.
 Definition f (n : nat) : term.
 
 Proof.
-intro n. destruct (eucl_dev k h0 n). exact (iter g q (nth r0)).
+intro n. destruct (eucl_dev k h0 n). exact (iter g q (nth r)).
 Defined.
 
 Require Import RelUtil.
@@ -163,19 +194,18 @@ Lemma IS_f : IS (red R) f.
 
 Proof.
 intro n; pattern n; apply lt_wf_ind; clear n; intros. unfold f at -2 .
-destruct (eucl_dev k h0 n); simpl. destruct (le_gt_dec (k-1) r0).
-(* r0 = k-1 *)
-assert (r0 = k-1). omega. assert (S n = (S q)*k + 0). rewrite mult_succ_l.
+destruct (eucl_dev k h0 n); simpl. destruct (le_gt_dec (k-1) r).
+(* r = k-1 *)
+assert (r = k-1). omega. assert (S n = (S q)*k + 0). rewrite mult_succ_l.
 omega. rewrite H1. unfold f. destruct (eucl_dev k h0 (S q * k + 0)).
 destruct (eucl_div_unique h0 g1 e0). rewrite <- H3. rewrite <- H2. simpl.
 apply red_iter_g. rewrite H0. fold last_term. rewrite last_term_g.
-apply red_g. unfold nth, list_terms.
-change (red R (List.nth 0 (t :: terms_of_reduc r) (Var 0))
-  (List.nth 1 (t :: terms_of_reduc r) (Var 0))).
-apply FS_red. destruct r. hyp. hyp.
-(* r0 < k-1 *)
-assert (S n = q*k + S r0). omega. rewrite H0. unfold f.
-destruct (eucl_dev k h0 (q * k + S r0)). assert (k>S r0). omega.
+apply red_g. unfold nth.
+change (red R (List.nth 0 (t :: us) (Var 0)) (List.nth 1 (t :: us) (Var 0))).
+apply FS_red. apply (rewrites_correct h1). hyp.
+(* r < k-1 *)
+assert (S n = q*k + S r). omega. rewrite H0. unfold f.
+destruct (eucl_dev k h0 (q * k + S r)). assert (k>S r). omega.
 destruct (eucl_div_unique H1 g2 e0). rewrite <- H3. rewrite <- H2.
 apply red_iter_g. apply FS_red'. omega.
 Qed.
@@ -193,4 +223,47 @@ unfold not. intro. eapply WF_notIS. apply fin_branch. apply h5. hyp.
 apply IS_f.
 Qed.
 
+End loop.
+
+(***********************************************************************)
+(** boolean function testing non-termination *)
+
+Definition is_loop t ds p :=
+  match rewrites t ds with
+    | None => false
+    | Some us =>
+      match us with
+        | nil => false
+        | _ =>
+          let u := last us (Var 0) in
+            match subterm_pos u p with
+              | None => false
+              | Some v =>
+                match matches t v with
+                  | None => false
+                  | Some _ => true
+                end
+            end
+      end
+  end.
+
+Lemma is_loop_correct : rules_preserv_vars R ->
+  forall t ds p, is_loop t ds p = true -> ~WF (red R).
+
+Proof.
+intros HR t ds p. unfold is_loop. coq_case_eq (rewrites t ds). 2: discr.
+destruct l. discr. set (us := t0::l). set (u := last us (Var 0)).
+coq_case_eq (subterm_pos u p). 2: discr. intro v. case_eq (matches t v).
+2: discr. eapply loop. apply H1. unfold k, us. simpl. omega.
+unfold last_term, k, nth. rewrite <- last_nth. fold u. apply H0. apply H. hyp.
+Qed.
+
 End S.
+
+(***********************************************************************)
+(** tactics *)
+
+Ltac loop t' ds' p' :=
+  rewrite red_mod_empty;
+  apply is_loop_correct with (t:=t') (ds:=ds') (p:=p');
+    [rules_preserv_vars | vm_compute; refl].
